src/Main.fsti
@@ -1,0 +1,206 @@
+module Main
+
+module U8 = FStar.UInt8
+module U32 = FStar.UInt32
+module U64 = FStar.UInt64
+module US = FStar.SizeT
+
+module TLA = Steel.TLArray
+
+open FStar.Mul
+open Steel.Effect.Atomic
+open Steel.Effect
+//open Steel.Array
+module A = Steel.Array
+//module R = Steel.Reference
+//module L = Steel.SpinLock
+module AL = ArrayList
+//module ALG = ArrayListGen
+//module SAA = Steel.ArrayArith
+
+//open Prelude
+//open SizeClass
+//open SteelVRefineDep
+//open SteelStarSeqUtils
+
+//open Utils2
+//open Mman
+
+val metadata_max_ex: US.t
+val slab_size: US.t
+val sc_slab_region_size: US.t
+
+open Constants
+open Config
+open SizeClass
+open Utils2
+
+noextract inline_for_extraction
+val init_struct_aux
+  (sc:sc)
+  (slab_region: array U8.t{A.length slab_region == U32.v page_size * US.v metadata_max})
+  (md_bm_region: array U64.t{A.length md_bm_region == US.v 4sz * US.v metadata_max})
+  (md_region: array AL.cell{A.length md_region == US.v metadata_max})
+  : Steel size_class_struct_sc
+  (
+    A.varray slab_region `star`
+    A.varray md_bm_region `star`
+    A.varray md_region
+  )
+  (fun scs -> size_class_vprop_sc scs)
+  (requires fun h0 ->
+    array_u8_alignment slab_region page_size /\
+    zf_u8 (A.asel slab_region h0) /\
+    zf_u64 (A.asel md_bm_region h0)
+  )
+  (ensures fun _ r h1 ->
+    r.size == Sc sc /\
+    //zf_u8 (A.asel (A.split_l slab_region (US.mul (US.mul metadata_max (u32_to_sz page_size)) (US.sub n 1sz))) h1) /\
+    //zf_u64 (A.asel (A.split_l md_bm_region (US.mul (US.mul metadata_max 4sz) (US.sub n 1sz))) h1) /\
+    r.slab_region == slab_region /\
+    r.md_bm_region == md_bm_region /\
+    r.md_region == md_region /\
+    True
+  )
+
+/// An attribute, that will indicate that the annotated functions should be unfolded at compile-time
+irreducible let reduce_attr : unit = ()
+
+open Mman
+
+//unfold
+val size_class_pred (slab_region:array U8.t) (sc:size_class) (i:nat) : prop
+
+module UP = FStar.PtrdiffT
+val slab_region_size
+  : v:US.t{
+    US.v v == US.v metadata_max * U32.v page_size * US.v nb_size_classes * US.v nb_arenas /\
+    UP.fits (US.v v)
+  }
+
+
+/// A logical predicate indicating that a list of sizes corresponds
+/// to the sizes of a list of size_classes
+val synced_sizes
+  //(nb_arenas: US.t)
+  //(n: US.t)
+  (offset: US.t)
+  (size_classes: Seq.seq size_class)
+  (sizes:TLA.t sc_union)
+  (k:nat{
+    k <= Seq.length size_classes /\
+    k + US.v offset <= TLA.length sizes
+  })
+  : prop
+
+//val hidden_pred
+//  (l1: list sc)
+//  (l2: list sc_ex)
+//  (n n1 n2 s1 s2 s3: US.t)
+//  : prop
+//
+//val hidden_pred2
+//  (n s1: US.t)
+//  : prop
+
+//noextract inline_for_extraction
+//val init_all_arenas
+//  (l1:list sc)
+//  (l2:list sc_ex)
+//  (n1 n2: US.t)
+//  (n: US.t{
+//    US.v n > 0 /\
+//    UInt.size (US.v n) U32.n /\
+//    True
+//    //US.fits (US.v n)
+//  })
+//  (arena_slab_region_size
+//   arena_md_region_size
+//   arena_md_bm_region_size
+//   arena_md_bm_region_b_size: (v:US.t{US.v v > 0}))
+//  (nb_arenas: US.t{US.v nb_arenas > 0 /\
+//    US.fits (US.v n * US.v nb_arenas) /\
+//    US.fits (US.v arena_slab_region_size * US.v nb_arenas) /\
+//    US.fits (US.v arena_md_bm_region_size * US.v nb_arenas) /\
+//    US.fits (US.v arena_md_bm_region_b_size * US.v nb_arenas) /\
+//    US.fits (US.v arena_md_region_size * US.v nb_arenas)
+//  })
+//  (slab_region: array U8.t{
+//    A.length slab_region == US.v arena_slab_region_size * US.v nb_arenas
+//  })
+//  (md_bm_region: array U64.t{
+//    A.length md_bm_region == US.v arena_md_bm_region_size * US.v nb_arenas
+//  })
+//  (md_bm_region_b: array bool{
+//    A.length md_bm_region_b == US.v arena_md_bm_region_b_size * US.v nb_arenas
+//  })
+//  (md_region: array AL.cell{
+//    A.length md_region == US.v arena_md_region_size * US.v nb_arenas
+//  })
+//  (size_classes: array size_class{
+//    A.length size_classes == US.v n * US.v nb_arenas
+//  })
+//  (sizes: TLA.t sc_union{
+//    TLA.length sizes == US.v n * US.v nb_arenas
+//  })
+//  : Steel unit
+//  (
+//    A.varray slab_region `star`
+//    A.varray md_bm_region `star`
+//    A.varray md_bm_region_b `star`
+//    A.varray md_region `star`
+//    A.varray size_classes
+//  )
+//  (fun _ ->
+//    A.varray size_classes
+//  )
+//  (requires fun h0 ->
+//    array_u8_alignment (A.split_r slab_region (US.mul arena_slab_region_size 0sz)) (u32_to_sz page_size) /\
+//    zf_u8 (A.asel slab_region h0) /\
+//    zf_u64 (A.asel md_bm_region h0) /\
+//    zf_b (A.asel md_bm_region_b h0) /\
+//    hidden_pred l1 l2 n n1 n2
+//      arena_md_bm_region_size
+//      arena_md_bm_region_b_size
+//      arena_md_region_size /\
+//    hidden_pred2 n arena_slab_region_size /\
+//    US.fits (US.v n * US.v nb_arenas) /\
+//    True
+//  )
+//  (ensures fun _ _ h1 ->
+//    hidden_pred2 n arena_slab_region_size /\
+//    US.fits (US.v n * US.v nb_arenas) /\
+//    synced_sizes 0sz
+//      (A.asel size_classes h1) sizes (US.v nb_arenas * US.v n) /\
+//    (forall (i:nat{i < US.v nb_arenas * US.v n}).
+//      size_class_pred slab_region (Seq.index (A.asel size_classes h1) i) i
+//    ) /\
+//    True
+//  )
+
+open NullOrVarray
+
+inline_for_extraction noextract
+val return_null ()
+  : Steel (array U8.t)
+  emp
+  (fun r -> null_or_varray r)
+  (requires fun _ -> True)
+  (ensures fun _ r _ -> A.is_null r)
+
+/// Wrapper around allocate_size_class, that does not return a pair, and instead
+/// always returns a valid permission on the new pointer if it is not null
+inline_for_extraction noextract
+val allocate_size_class
+  (scs: size_class_struct)
+  : Steel (array U8.t)
+  (size_class_vprop scs)
+  (fun r -> null_or_varray r `star` size_class_vprop scs)
+  (requires fun h0 -> True)
+  (ensures fun h0 r h1 ->
+    not (A.is_null r) ==> (
+      A.length r == U32.v (get_u32 scs.size) /\
+      array_u8_alignment r 16ul /\
+      ((U32.v (get_u32 scs.size) > 0 /\ (U32.v page_size) % (U32.v (get_u32 scs.size)) == 0) ==> array_u8_alignment r (get_u32 scs.size))
+    )
+  )
